---
title: COMP-2310 Formula Cheatsheet
date: 2022-09-04
draft: false
---

Contained here are the main equivalences and inference rules for the COMP-2310 class at UWindsor.

*Yes I know the latex is not currently rendering on this page, I hope to fix it soon*

## Equivalences

E1. \\( \alpha \land \sim \alpha \equiv false \\)  
E2. \\( \alpha \lor \sim \alpha \equiv true \\)  
E3. \\( \alpha \land \alpha \equiv \alpha \\)  
E4. \\( \alpha \lor \alpha \equiv \alpha \\)  
E5. \\( \alpha \land true \equiv \alpha \\)  
E6. \\( \alpha \lor false \equiv \alpha \\)  
E7. \\( \alpha \land false \equiv false \\)  
E8. \\( \alpha \lor true \equiv true \\)  
E9. \\( \alpha \land \beta \equiv \beta \land \alpha \\)  
E10. \\( \alpha \lor \beta \equiv \beta \lor \alpha \\)  
E11. \\( (\alpha \land \beta) \land \gamma \equiv \alpha \land (\beta \land \gamma) \\)  
E12. \\( (\alpha \lor \beta) \lor \gamma \equiv \alpha \lor (\beta \lor \gamma) \\)  
E13. \\( \alpha \land (\beta \lor \gamma) \equiv (\alpha \land \beta) \lor (\alpha \land \gamma) \\)  
E14. \\( \alpha \lor (\beta \land \gamma) \equiv (\alpha \lor \beta) \land (\alpha \lor \gamma) \\)  
E15. \\( \sim \sim \alpha \equiv \alpha \\)  
E16. \\( \sim (\alpha \land \beta) \equiv (\sim \alpha \lor \sim \beta) \\)  
E17. \\( \sim (\alpha \lor \beta) \equiv (\sim \alpha \land \sim \beta) \\)  
E18. \\( \alpha \implies \beta \equiv \sim \alpha \lor \beta \\)  
E19. \\( \alpha \implies \beta \equiv \sim \beta \implies \sim \alpha \\)  
E20. \\( (\alpha \implies \beta) \land (\beta \implies \alpha) \equiv \alpha \iff \beta \\)  

## Inference Rules

#### I1. \\( \frac{p}{p \lor q} \\)  
#### I2. \\( \frac{p \land q}{p} \\)  
#### I3. \\( \frac{p, p \implies q}{q} \\)  
#### I4. \\( \frac{\sim q, p \implies q}{\sim p} \\)  
#### I5. \\( \frac{p \implies q, q \implies r}{p \implies r} \\)  
#### I6. \\( \frac{p, q}{p \land q} \\)  

## First-Order Logic Equivalences

FE1. \\( (\forall x)\alpha(x) \equiv (\forall y)\alpha(y) \quad (\alpha(x) \text{ does not contain } y) \\)  
FE2. \\( (\exists x)\alpha(x) \equiv (\exists y)\alpha(y) \quad (\alpha(x) \text{ does not contain } y) \\)  
FE3. \\( (\forall x)\alpha(x) \lor \beta \equiv (\forall x)(\alpha(x) \lor \beta) \quad (\beta \text{ contains no free occurrence of } x) \\)  
FE4. \\( (\exists x)\alpha(x) \lor \beta \equiv (\exists x)(\alpha(x) \lor \beta) \quad (\beta \text{ contains no free occurrence of } x) \\)  
FE5. \\( (\forall x)\alpha(x) \land \beta \equiv (\forall x)(\alpha(x) \land \beta) \quad (\beta \text{ contains no free occurrence of } x) \\)  
FE6. \\( (\exists x)\alpha(x) \land \beta \equiv (\exists x)(\alpha(x) \land \beta) \quad (\beta \text{ contains no free occurrence of } x) \\)  
FE7. \\( \sim (\forall x)\alpha(x) \equiv (\exists x)\sim \alpha(x) \\)  
FE8. \\( \sim (\exists x)\alpha(x) \equiv (\forall x)\sim \alpha(x) \\)  
FE9. \\( (\forall x)\alpha(x) \land (\forall x)\beta(x) \equiv (\forall x)(\alpha(x) \land \beta(x)) \\)  
FE10. \\( (\exists x)\alpha(x) \lor (\exists x)\beta(x) \equiv (\exists x)(\alpha(x) \lor \beta(x)) \\)  

## First-Order Logic Inference Rules

#### **Gen**: Generalization  
#### \\( \frac{\alpha(x)}{(\forall x)\alpha(x)} \\)  
\\( x \text{ is a variable} \\)  

#### **UI**: Universal Instantiation  
#### \\( \frac{(\forall x)\alpha(x)}{\alpha(t)} \\)  
\\( \alpha(x) \text{ is free for } t \text{ (} t \text{ is a variable or constant)} \\)  
\\( \text {where }\alpha(t) \text{ results from } \alpha(x) \text{ after all free occurrences of x in } \alpha(x) \text{ are replaced by } t \\)  

#### **EQ**: Existential Quantification  
#### \\( \frac{\alpha(t)}{(\exists x)\alpha(x)} \\)  
\\( \alpha(x) \text{ is free for } t \text{ (} t \text{ is a variable or constant)} \\)  
\\( \text {where }\alpha(x) \text{ results from } \alpha(t) \text{ after some (may be all) free occurences of t in } \alpha(t) \text{ are replaced by } x \\)  
